Extract tip of nominal_datatype to be new atom_type branch.
This work doesn't build yet, but this commit makes the history nicer
because the work now builds on the 'known good' perm_type.

examples/lambda/basics/NEWLib.sml
@@ -3,17 +3,18 @@ struct
 
 open HolKernel boolLib BasicProvers simpLib basic_swapTheory
 
-val string_ty = stringSyntax.string_ty
-val strset_finite_t = inst [alpha |-> string_ty] pred_setSyntax.finite_tm
-fun NEW_TAC vname t (asl, g) = let
-  val var = mk_var(vname, string_ty)
+val atom_ty = mk_thy_type {Thy="basic_swap",Args=[],Tyop="atom"}
+val atomset_finite_t = inst [alpha |-> atom_ty] pred_setSyntax.finite_tm
+fun NEW_TAC vname sort_tm (asl, g) = let
+  val var = mk_var(vname, atom_ty)
   open pred_setTheory
+  val (sort,tm) = pairSyntax.dest_pair sort_tm
   val fresh_thm =
       (CONV_RULE (RAND_CONV (REWRITE_CONV [IN_INSERT, IN_UNION, DE_MORGAN_THM,
                                            NOT_IN_EMPTY])) o
-       SPEC t) new_exists
-  fun is_finitestrset t = free_in strset_finite_t t
-  val finite_asms = filter is_finitestrset asl
+       SPECL [tm,sort]) new_exists
+  fun is_finite_atomset t = free_in atomset_finite_t t
+  val finite_asms = filter is_finite_atomset asl
   val finiteness_discharged0 =
       CONV_RULE (LAND_CONV (SIMP_CONV (srw_ss()) (map ASSUME finite_asms)))
                 fresh_thm
@@ -33,7 +34,7 @@ end (asl, g)
    ---------------------------------------------------------------------- *)
 
 fun NEW_ELIM_TAC (asl, w) = let
-  val newt = find_term (can (match_term ``NEW (X:string set)``)) w
+  val newt = find_term (can (match_term ``NEW A s``)) w
 in
   CONV_TAC (UNBETA_CONV newt) THEN MATCH_MP_TAC NEW_ELIM_RULE THEN
   SIMP_TAC (srw_ss()) []
